<?xml version="1.0"?>


<!DOCTYPE rdf:RDF [
    <!ENTITY owl "http://www.w3.org/2002/07/owl#" >
    <!ENTITY xsd "http://www.w3.org/2001/XMLSchema#" >
    <!ENTITY rdfs "http://www.w3.org/2000/01/rdf-schema#" >
    <!ENTITY rdf "http://www.w3.org/1999/02/22-rdf-syntax-ns#" >
]>


<rdf:RDF xmlns="http://www.semanticweb.org/GRISERA/contextualOntology/configurations/ssn-noninvasive#"
     xml:base="http://www.semanticweb.org/GRISERA/contextualOntology/configurations/ssn-noninvasive"
     xmlns:rdfs="http://www.w3.org/2000/01/rdf-schema#"
     xmlns:owl="http://www.w3.org/2002/07/owl#"
     xmlns:xsd="http://www.w3.org/2001/XMLSchema#"
     xmlns:rdf="http://www.w3.org/1999/02/22-rdf-syntax-ns#">
    <owl:Ontology rdf:about="http://www.semanticweb.org/GRISERA/contextualOntology/configurations/ssn-noninvasive">
        <owl:imports rdf:resource="http://www.semanticweb.org/GRISERA/contextualOntology/configurations"/>
        <owl:imports rdf:resource="http://www.w3.org/ns/ssn/systems/"/>
    </owl:Ontology>
    


    <!-- 
    ///////////////////////////////////////////////////////////////////////////////////////
    //
    // Object Properties
    //
    ///////////////////////////////////////////////////////////////////////////////////////
     -->

    


    <!-- http://www.semanticweb.org/GRISERA/contextualOntology/configurations/ssn-noninvasive#forSSNproperty -->

    <owl:ObjectProperty rdf:about="http://www.semanticweb.org/GRISERA/contextualOntology/configurations/ssn-noninvasive#forSSNproperty">
        <rdfs:comment xml:lang="en">An object property allowing to specify a SSN property which exists under a SSN certain condition.</rdfs:comment>
        <rdfs:subPropertyOf rdf:resource="http://www.semanticweb.org/GRISERA/contextualOntology/configurations#forProperty"/>
        <rdfs:subPropertyOf rdf:resource="http://www.w3.org/ns/ssn/forProperty"/>
    </owl:ObjectProperty>
    


    <!-- http://www.semanticweb.org/GRISERA/contextualOntology/configurations/ssn-noninvasive#inSSNCondition -->

    <owl:ObjectProperty rdf:about="http://www.semanticweb.org/GRISERA/contextualOntology/configurations/ssn-noninvasive#inSSNCondition">
        <rdfs:comment xml:lang="en">An object property allowing to specify a condition under which a property exists.</rdfs:comment>
        <rdfs:subPropertyOf rdf:resource="http://www.semanticweb.org/GRISERA/contextualOntology/configurations#inCondition"/>
        <rdfs:subPropertyOf rdf:resource="http://www.w3.org/ns/ssn/systems/inCondition"/>
    </owl:ObjectProperty>
    


    <!-- 
    ///////////////////////////////////////////////////////////////////////////////////////
    //
    // Classes
    //
    ///////////////////////////////////////////////////////////////////////////////////////
     -->

    


    <!-- http://www.semanticweb.org/GRISERA/contextualOntology/configurations/ssn-noninvasive#ConfiguredOperatingRange -->

    <owl:Class rdf:about="http://www.semanticweb.org/GRISERA/contextualOntology/configurations/ssn-noninvasive#ConfiguredOperatingRange">
        <rdfs:subClassOf rdf:resource="http://www.semanticweb.org/GRISERA/contextualOntology/configurations#Configuration"/>
        <rdfs:subClassOf rdf:resource="http://www.w3.org/ns/ssn/systems/OperatingRange"/>
        <rdfs:comment xml:lang="en">Describes an element of ROAD configuration, which is described as SSN operating range.</rdfs:comment>
    </owl:Class>
    


    <!-- http://www.semanticweb.org/GRISERA/contextualOntology/configurations/ssn-noninvasive#ConfiguredSystemCapability -->

    <owl:Class rdf:about="http://www.semanticweb.org/GRISERA/contextualOntology/configurations/ssn-noninvasive#ConfiguredSystemCapability">
        <rdfs:subClassOf rdf:resource="http://www.semanticweb.org/GRISERA/contextualOntology/configurations#Configuration"/>
        <rdfs:subClassOf rdf:resource="http://www.w3.org/ns/ssn/systems/SystemCapability"/>
        <rdfs:comment xml:lang="en">Describes an element of ROAD configuration, which is described as SSN system capability.</rdfs:comment>
    </owl:Class>
</rdf:RDF>



<!-- Generated by the OWL API (version 3.4.2) http://owlapi.sourceforge.net -->

