<?xml version="1.0"?>


<!DOCTYPE rdf:RDF [
    <!ENTITY owl "http://www.w3.org/2002/07/owl#" >
    <!ENTITY xsd "http://www.w3.org/2001/XMLSchema#" >
    <!ENTITY rdfs "http://www.w3.org/2000/01/rdf-schema#" >
    <!ENTITY rdf "http://www.w3.org/1999/02/22-rdf-syntax-ns#" >
]>


<rdf:RDF xmlns="http://www.semanticweb.org/GRISERA/contextualOntology/configurations#"
     xml:base="http://www.semanticweb.org/GRISERA/contextualOntology/configurations"
     xmlns:rdfs="http://www.w3.org/2000/01/rdf-schema#"
     xmlns:owl="http://www.w3.org/2002/07/owl#"
     xmlns:xsd="http://www.w3.org/2001/XMLSchema#"
     xmlns:rdf="http://www.w3.org/1999/02/22-rdf-syntax-ns#">
    <owl:Ontology rdf:about="http://www.semanticweb.org/GRISERA/contextualOntology/configurations">
        <owl:imports rdf:resource="http://www.semanticweb.org/GRISERA/contextualOntology"/>
    </owl:Ontology>
    


    <!-- 
    ///////////////////////////////////////////////////////////////////////////////////////
    //
    // Object Properties
    //
    ///////////////////////////////////////////////////////////////////////////////////////
     -->

    


    <!-- http://www.semanticweb.org/GRISERA/contextualOntology/configurations#forProperty -->

    <owl:ObjectProperty rdf:about="http://www.semanticweb.org/GRISERA/contextualOntology/configurations#forProperty">
        <rdfs:comment xml:lang="en">An object property allowing to specify a property which exists under a certain condition.</rdfs:comment>
        <rdfs:domain rdf:resource="http://www.semanticweb.org/GRISERA/contextualOntology/configurations#Configuration"/>
        <rdfs:range rdf:resource="http://www.semanticweb.org/GRISERA/contextualOntology/configurations#ConfigurationProperty"/>
    </owl:ObjectProperty>
    


    <!-- http://www.semanticweb.org/GRISERA/contextualOntology/configurations#inCondition -->

    <owl:ObjectProperty rdf:about="http://www.semanticweb.org/GRISERA/contextualOntology/configurations#inCondition">
        <rdfs:comment xml:lang="en">An object property allowing to specify a condition under which a property exists.</rdfs:comment>
        <rdfs:domain rdf:resource="http://www.semanticweb.org/GRISERA/contextualOntology/configurations#Configuration"/>
        <rdfs:range rdf:resource="http://www.semanticweb.org/GRISERA/contextualOntology/configurations#InConfigurationCondition"/>
    </owl:ObjectProperty>
    


    <!-- http://www.semanticweb.org/GRISERA/contextualOntology/configurations#isConfigurationConditionOf -->

    <owl:ObjectProperty rdf:about="http://www.semanticweb.org/GRISERA/contextualOntology/configurations#isConfigurationConditionOf">
        <rdf:type rdf:resource="&owl;FunctionalProperty"/>
        <rdfs:comment xml:lang="en">An object property allowing to specify a condition (or a set of conditions) that are specific for a certain configuration source.</rdfs:comment>
        <rdfs:range rdf:resource="http://www.semanticweb.org/GRISERA/contextualOntology/configurations#ConfigurationSource"/>
        <rdfs:domain rdf:resource="http://www.semanticweb.org/GRISERA/contextualOntology/configurations#InConfigurationCondition"/>
    </owl:ObjectProperty>
    


    <!-- 
    ///////////////////////////////////////////////////////////////////////////////////////
    //
    // Classes
    //
    ///////////////////////////////////////////////////////////////////////////////////////
     -->

    


    <!-- http://www.semanticweb.org/GRISERA/contextualOntology#Channel -->

    <rdf:Description rdf:about="http://www.semanticweb.org/GRISERA/contextualOntology#Channel">
        <rdfs:subClassOf rdf:resource="http://www.semanticweb.org/GRISERA/contextualOntology/configurations#ConfigurationSource"/>
    </rdf:Description>
    


    <!-- http://www.semanticweb.org/GRISERA/contextualOntology#Recording -->

    <rdf:Description rdf:about="http://www.semanticweb.org/GRISERA/contextualOntology#Recording">
        <rdfs:subClassOf rdf:resource="http://www.semanticweb.org/GRISERA/contextualOntology/configurations#ConfigurationSource"/>
    </rdf:Description>
    


    <!-- http://www.semanticweb.org/GRISERA/contextualOntology#RegisteredChannel -->

    <rdf:Description rdf:about="http://www.semanticweb.org/GRISERA/contextualOntology#RegisteredChannel">
        <rdfs:subClassOf rdf:resource="http://www.semanticweb.org/GRISERA/contextualOntology/configurations#ConfigurationSource"/>
    </rdf:Description>
    


    <!-- http://www.semanticweb.org/GRISERA/contextualOntology/configurations#Configuration -->

    <owl:Class rdf:about="http://www.semanticweb.org/GRISERA/contextualOntology/configurations#Configuration">
        <rdfs:subClassOf>
            <owl:Restriction>
                <owl:onProperty rdf:resource="http://www.semanticweb.org/GRISERA/contextualOntology/configurations#forProperty"/>
                <owl:someValuesFrom rdf:resource="&owl;Thing"/>
            </owl:Restriction>
        </rdfs:subClassOf>
        <rdfs:subClassOf>
            <owl:Restriction>
                <owl:onProperty rdf:resource="http://www.semanticweb.org/GRISERA/contextualOntology/configurations#inCondition"/>
                <owl:someValuesFrom rdf:resource="&owl;Thing"/>
            </owl:Restriction>
        </rdfs:subClassOf>
        <rdfs:comment xml:lang="en">Describes an element of configuration, which is understood as existence of partiular configuration property under certain condition.</rdfs:comment>
    </owl:Class>
    


    <!-- http://www.semanticweb.org/GRISERA/contextualOntology/configurations#ConfigurationProperty -->

    <owl:Class rdf:about="http://www.semanticweb.org/GRISERA/contextualOntology/configurations#ConfigurationProperty">
        <rdfs:comment xml:lang="en">Describes a particular configuration property of interest (an identifiable and observable characteristic of anything in the scope of an experiment).</rdfs:comment>
    </owl:Class>
    


    <!-- http://www.semanticweb.org/GRISERA/contextualOntology/configurations#ConfigurationSource -->

    <owl:Class rdf:about="http://www.semanticweb.org/GRISERA/contextualOntology/configurations#ConfigurationSource">
        <rdfs:comment xml:lang="en">Objects that can be a source of configuration for execution of an experiment or a part of an experiment</rdfs:comment>
    </owl:Class>
    


    <!-- http://www.semanticweb.org/GRISERA/contextualOntology/configurations#InConfigurationCondition -->

    <owl:Class rdf:about="http://www.semanticweb.org/GRISERA/contextualOntology/configurations#InConfigurationCondition">
        <rdfs:subClassOf>
            <owl:Restriction>
                <owl:onProperty rdf:resource="http://www.semanticweb.org/GRISERA/contextualOntology/configurations#isConfigurationConditionOf"/>
                <owl:someValuesFrom rdf:resource="&owl;Thing"/>
            </owl:Restriction>
        </rdfs:subClassOf>
        <rdfs:comment xml:lang="en">Describes a state in which particular configuration properties exist.</rdfs:comment>
    </owl:Class>
</rdf:RDF>



<!-- Generated by the OWL API (version 3.4.2) http://owlapi.sourceforge.net -->

